sap 5

lab5/lab5.dfy
@@ -38,3 +38,133 @@ function sumBetween(a: int, b: int) : int
   else
     a + sumBetween(a + 1, b)
 }
+
+//ex 3
+ghost function fib_axiomatized(n: int) : int
+
+lemma fib_axiomatized0()
+  ensures fib_axiomatized(0) == 0
+
+lemma fib_axiomatized1()
+  ensures fib_axiomatized(1) == 1
+
+lemma fib_axiomatizedRec(n: int)
+  requires n > 1
+  ensures fib_axiomatized(n) == fib_axiomatized(n - 1) + fib_axiomatized(n - 2)
+
+function fib_defined(n: int) : int
+  requires n >= 0
+  decreases n
+{
+  if n == 0 then
+    0
+  else if n == 1 then
+    1
+  else
+    fib_defined(n - 1) + fib_defined(n - 2)
+}
+
+lemma equivalenceFib(n: int)
+  requires n >= 0
+  ensures fib_axiomatized(n) == fib_defined(n)
+{
+  if n == 0 {
+    fib_axiomatized0();
+    assert fib_axiomatized(0) == 0;
+  } else if n == 1 {
+    fib_axiomatized1();
+    assert fib_axiomatized(1) == 1;
+  } else {
+    if n > 1 {
+      fib_axiomatizedRec(n);
+      equivalenceFib(n - 1);
+      equivalenceFib(n - 2);
+      assert fib_axiomatized(n) == fib_axiomatized(n - 1) + fib_axiomatized(n - 2);
+      assert fib_axiomatized(n) == fib_defined(n - 1) + fib_defined(n - 2);
+    }
+  }
+}
+
+// ex 4
+type BST(0) 
+
+ghost const Leaf : BST
+
+ghost function Node(x: int, l: BST, r: BST) : BST
+
+lemma node_injective(n1: int, l1: BST, r1: BST, n2: int, l2: BST, r2: BST)
+  requires Node(n1, l1, r1) == Node(n2, l2, r2)
+  ensures n1 == n2 && l1 == l2 && r1 == r2
+
+lemma node_leaf_distinct(n: int, l: BST, r: BST)
+  ensures Node(n, l, r) != Leaf
+
+lemma bst_total(t: BST)
+  ensures t == Leaf || exists n: int, l: BST, r: BST :: t == Node(n, l, r)
+
+lemma inductionBST(P: BST -> bool)
+  requires P(Leaf) 
+  requires forall n: int, l: BST, r: BST :: P(l) && P(r) ==> P(Node(n, l, r)) 
+  ensures forall t: BST :: P(t)
+
+ghost function IsLeaf(t: BST) : bool
+ghost function IsNode(t: BST) : bool
+
+lemma leaf_node_total(t: BST)
+  ensures IsLeaf(t) || IsNode(t)
+
+lemma leaf_node_exclusivity(t: BST)
+  ensures IsLeaf(t) ==> !IsNode(t) && IsNode(t) ==> !IsLeaf(t)
+
+ghost function GetValue(t: BST) : int
+  requires IsNode(t)
+
+ghost function GetLeft(t: BST) : BST
+  requires IsNode(t)
+
+ghost function GetRight(t: BST) : BST
+  requires IsNode(t)
+
+lemma node_accessors(n: int, l: BST, r: BST)
+  ensures IsNode(Node(n, l, r)) 
+  ensures GetValue(Node(n, l, r)) == n
+  ensures GetLeft(Node(n, l, r)) == l
+  ensures GetRight(Node(n, l, r)) == r
+
+
+//ex 5
+predicate isDivisorFunctional(x: int, y: int)
+  requires x > 0 && y >= 0
+{
+  y % x == 0
+}
+predicate isDivisorQuantified(x: int, y: int)
+    requires x>1 && y>1
+{
+    exists k: int :: 0 <= k <= y && y == x * k
+}
+
+//ex 6
+ghost predicate isGCD(d: int, a: int, b: int)
+    requires a >= 0 && b >= 0
+{
+    if a == 0 && b == 0 then
+        d == 0
+    else
+        d > 0 &&
+        exists k1: int :: k1 >= 0 && a == d * k1 &&
+        exists k2: int :: k2 >= 0 && b == d * k2 &&
+        forall e: int ::
+            (e > 0 && exists k3: int :: (k3 >= 0 && a == e * k3) && exists k4: int :: (k4 >= 0 && b == e * k4)) ==> (e <= d)
+}
+
+//ex 7
+function gcd(a: int, b: int) : int
+  requires a >= 0 && b >= 0
+  decreases b
+{
+  if b == 0 then
+    a
+  else
+    gcd(b, a % b)
+}
